building separation logic in LamRefLogicFacts.v

src/LambdaAssertions.v
@@ -53,3 +53,24 @@ Definition hoare_triple {V : Set}
   forall (v : Value V) (c : nat) (m m' : Map V),
     C[e, m ~~> v, m' | c] ->
     P m -> Q v c m'.
+
+(*
+(* total correctness *)
+(* hoare triple for one step of reduction *)
+Definition step_hoare_triple {V : Set}
+  (e : Expr V) (P Q : StateAssertion V) : Prop :=
+  forall (e' : Expr V) (m m' : Map V),
+    P m ->
+    exists (m' : Map V),
+      R[e, m ~~> e', m'] ->
+      Q m.
+
+Definition hoare_triple {V : Set}
+  (e : Expr V)
+  (P : StateAssertion V) (Q : Value V -> nat -> StateAssertion V) : Prop :=
+  forall (v : Value V) (m : Map V),
+    P m ->
+    exists (c : nat) (m' : Map V),
+      C[e, m ~~> v, m' | c] ->
+      Q v c m'.
+*)
