src/Example2.v
@@ -8,56 +8,56 @@ Require Import src.Tactics.
 Definition e : Expr Empty_set := (
   -\ -\ Ref (Var ($ None) <* ! Var None)
 ).
-
+(*
 (* e typechecks *)
 Fact type_e (t1 t2 : type) :
   T[ env_empty |- e ::: (t1 --> t2) --> (RefT t1) --> (RefT t2) ].
 Proof.
   solve_typing.
 Qed.
-
+*)
 (* map for Ref in place *)
 Definition e' : Expr Empty_set := (
   -\ -\ Var None <- (Var ($ None) <* ! Var None)
 ).
-
+(*
 (* e' typechecks *)
 Fact type_e' (t : type) :
   T[ env_empty |- e' ::: (t --> t) --> (RefT t) --> Unit ].
 Proof.
   solve_typing.
 Qed.
-
+*)
 Definition e_id : Expr Empty_set := (
   -\ Var None
 ).
-
+(*
 (* e_id typechecks *)
 Fact type_e_id (t : type) :
   T[ env_empty |- e_id ::: t --> t ].
 Proof.
   solve_typing.
 Qed.
-
+*)
 Definition e_ref_u : Expr Empty_set := (
   Ref U_val
 ).
-
+(*
 (* e_ref_u typechecks *)
 Fact type_e_ref_u : T[ env_empty |- e_ref_u ::: RefT Unit ].
 Proof.
   solve_typing.
 Qed.
-
+*)
 (* -------------------------------------------------------- *)
 
 Definition ex : Expr Empty_set := e <* e_id <* e_ref_u.
-
+(*
 Fact type_ex : T[ env_empty |- ex ::: RefT Unit ].
 Proof.
   solve_typing.
 Qed.
-
+*)
 Goal exists l m c,
   cost_red ex []%list (Lab l) m c /\
   List.In (l, U_val) m.
@@ -86,20 +86,20 @@ Proof.
 Qed.
 
 Definition ex' : Expr Empty_set := e' <* e_id <* e_ref_u.
-
+(*
 Fact type_ex' : T[ env_empty |- ex' ::: Unit ].
 Proof.
   solve_typing.
 Qed.
-
+*)
 Definition ex'' : Expr Empty_set :=
   (-\ shift_e e' <* shift_e e_id <* Var None ;; Var None) <* e_ref_u.
-
+(*
 Fact type_ex'' : T[ env_empty |- ex'' ::: RefT Unit ].
 Proof.
   solve_typing.
 Qed.
-
+*)
 Goal exists l m c,
   cost_red ex'' []%list (Lab l) m c /\
   List.In (l, U_val) m.
