src/Example4.v
@@ -26,14 +26,14 @@ Definition cons : Value string :=
           Var "xs"
         ]
   )%string.
-
+(*
 Fact cons_type :
   forall G n,
     T[ G |- cons ::: IntT --> fl_type n --> fl_type (S n)].
 Proof.
   solve_typing.
 Qed.
-
+*)
 Fixpoint finite_list_value {V : Set} (n : nat) : Value V :=
   match n with
   | 0 => U_val
@@ -42,7 +42,7 @@ Fixpoint finite_list_value {V : Set} (n : nat) : Value V :=
     finite_list_value n'
   ]
   end.
-
+(*
 Goal forall V G n,
   T[ G |- finite_list_value (V := V) n ::: fl_type n ].
 Proof.
@@ -50,13 +50,13 @@ Proof.
   - solve_typing.
   - cbn. repeat constructor. assumption.
 Qed.
-
+*)
 Fixpoint finite_list_expr (n : nat) : Expr string :=
   match n with
   | 0 => U_val
   | S n' => cons <* Int 0 <* finite_list_expr n'
   end.
-
+(*
 Goal forall G n,
   T[ G |- finite_list_expr n ::: fl_type n ].
 Proof.
@@ -68,7 +68,7 @@ Proof.
       * constructor.
     + assumption.
 Qed.
-
+*)
 Goal forall n m,
   exists c, C[finite_list_expr n, m ~~> finite_list_value n, m | c].
 Proof.
