src/LamRefLogicFacts.v
@@ -1,3 +1,4 @@
+Require Arith.
 Require List.
 Import List.ListNotations.
 Require Import String.
@@ -6,6 +7,33 @@ Require Import ZArith.
 Require Import src.LambdaRef.
 Require Import src.LamRefFacts.
 Require Import src.LambdaAssertions.
+
+(*
+(*total correctness*)
+Theorem triple_weaken (V : Set) (e : Expr V) P P' Q Q' :
+  sa_implies P' P ->
+  (forall v c, sa_implies (Q v c) (Q' v c)) ->
+  hoare_triple e P Q ->
+  hoare_triple e P' Q'.
+Proof.
+  unfold hoare_triple, sa_implies. intros HP HQ Hhoare v m p'.
+  edestruct Hhoare as [? [? ?]]; eauto.
+Qed.
+
+Theorem triple_value (V : Set) (v : Value V) (P : StateAssertion V) :
+  hoare_triple v P (fun _ c => sa_star (sa_pure (c = 0)) P).
+Proof.
+  unfold hoare_triple, sa_star, sa_pure, sa_empty, disjoint_maps.
+  intros v' m p. repeat eexists; eauto.
+Qed.
+
+Theorem triple_value' (V : Set) (v : Value V) :
+  hoare_triple v sa_empty (fun _ c => sa_pure (c = 0)).
+Proof.
+  unfold hoare_triple, sa_pure, sa_empty.
+  intros v' m p. repeat eexists.
+Qed.
+*)
 
 Theorem triple_weaken (V : Set) (e : Expr V) P P' Q Q' :
   sa_implies P' P ->
@@ -60,3 +88,266 @@ Proof.
   inversion Hred. subst. inversion H; subst; try discriminate_red_Val.
   inversion H0; subst; auto. discriminate_red_Val.
 Qed.
+
+Theorem triple_ineg (V : Set) (i : Z) :
+  @hoare_triple V ([--] Int i)
+    sa_empty
+    (fun v c => sa_pure (v = Int (- i) /\ c = 1)).
+Proof.
+  unfold hoare_triple, sa_pure, sa_empty. intros v c m m' Hred p.
+  inversion Hred. subst. inversion H; subst; try discriminate_red_Val.
+  inversion H0; subst; auto. discriminate_red_Val.
+Qed.
+
+Theorem triple_bor (V : Set) (b1 b2 : bool) :
+  @hoare_triple V ((Bool b1) [||] (Bool b2))
+    sa_empty
+    (fun v c => sa_pure (v = Bool (b1 || b2) /\ c = 1)).
+Proof.
+  unfold hoare_triple, sa_pure, sa_empty. intros v c m m' Hred p.
+  inversion Hred. subst. inversion H; subst; try discriminate_red_Val.
+  inversion H0; subst; auto. discriminate_red_Val.
+Qed.
+
+Theorem triple_band (V : Set) (b1 b2 : bool) :
+  @hoare_triple V ((Bool b1) [&&] (Bool b2))
+    sa_empty
+    (fun v c => sa_pure (v = Bool (b1 && b2) /\ c = 1)).
+Proof.
+  unfold hoare_triple, sa_pure, sa_empty. intros v c m m' Hred p.
+  inversion Hred. subst. inversion H; subst; try discriminate_red_Val.
+  inversion H0; subst; auto. discriminate_red_Val.
+Qed.
+
+Theorem triple_iadd (V : Set) (i1 i2 : Z) :
+  @hoare_triple V (Int i1 [+] Int i2)
+    sa_empty
+    (fun v c => sa_pure (v = Int (i1 + i2) /\ c = 1)).
+Proof.
+  unfold hoare_triple, sa_pure, sa_empty. intros v c m m' Hred p.
+  inversion Hred. subst. inversion H; subst; try discriminate_red_Val.
+  inversion H0; subst; auto. discriminate_red_Val.
+Qed.
+
+Theorem triple_isub (V : Set) (i1 i2 : Z) :
+  @hoare_triple V (Int i1 [-] Int i2)
+    sa_empty
+    (fun v c => sa_pure (v = Int (i1 - i2) /\ c = 1)).
+Proof.
+  unfold hoare_triple, sa_pure, sa_empty. intros v c m m' Hred p.
+  inversion Hred. subst. inversion H; subst; try discriminate_red_Val.
+  inversion H0; subst; auto. discriminate_red_Val.
+Qed.
+
+Theorem triple_imul (V : Set) (i1 i2 : Z) :
+  @hoare_triple V (Int i1 [*] Int i2)
+    sa_empty
+    (fun v c => sa_pure (v = Int (i1 * i2) /\ c = 1)).
+Proof.
+  unfold hoare_triple, sa_pure, sa_empty. intros v c m m' Hred p.
+  inversion Hred. subst. inversion H; subst; try discriminate_red_Val.
+  inversion H0; subst; auto. discriminate_red_Val.
+Qed.
+
+Theorem triple_idiv (V : Set) (i1 i2 : Z) :
+  @hoare_triple V (Int i1 [/] Int i2)
+    sa_empty
+    (fun v c => sa_pure (v = Int (i1 / i2) /\ c = 1)).
+Proof.
+  unfold hoare_triple, sa_pure, sa_empty. intros v c m m' Hred p.
+  inversion Hred. subst. inversion H; subst; try discriminate_red_Val.
+  inversion H0; subst; auto. discriminate_red_Val.
+Qed.
+
+Theorem triple_clt (V : Set) (i1 i2 : Z) :
+  @hoare_triple V (Int i1 [<] Int i2)
+    sa_empty
+    (fun v c => sa_pure (v = Bool (i1 <? i2)%Z /\ c = 1)).
+Proof.
+  unfold hoare_triple, sa_pure, sa_empty. intros v c m m' Hred p.
+  inversion Hred. subst. inversion H; subst; try discriminate_red_Val.
+  inversion H0; subst; auto. discriminate_red_Val.
+Qed.
+
+Theorem triple_ceq (V : Set) (i1 i2 : Z) :
+  @hoare_triple V (Int i1 [=] Int i2)
+    sa_empty
+    (fun v c => sa_pure (v = Bool (i1 =? i2)%Z /\ c = 1)).
+Proof.
+  unfold hoare_triple, sa_pure, sa_empty. intros v c m m' Hred p.
+  inversion Hred. subst. inversion H; subst; try discriminate_red_Val.
+  inversion H0; subst; auto. discriminate_red_Val.
+Qed.
+
+Theorem triple_rec_e2v (V : Set) (vs : list (Value V)) :
+  hoare_triple (RecE (vals2exprs vs))
+    sa_empty
+    (fun v c => sa_pure (v = RecV vs /\ c = 1)).
+Proof.
+  unfold hoare_triple, sa_pure, sa_empty. intros v c m m' Hred p.
+  inversion Hred. subst. inversion H; subst.
+  - apply vals2exprs_inj in H2. subst. inversion H0; subst; auto.
+    discriminate_red_Val.
+  - apply SplitAt_spec_eq in H2. unfold vals2exprs in *.
+    apply List.map_eq_app in H2 as [? [? [? [? ?]]]].
+    destruct x0; try discriminate; simpl in *. injection H5 as ? ?. subst.
+    discriminate_red_Val.
+Qed.
+
+Theorem triple_get (V : Set) (n : nat) (vs : list (Value V)) v :
+  Nth n vs v ->
+  @hoare_triple V (Get n (RecV vs))
+    sa_empty
+    (fun v' c => sa_pure (v' = v /\ c = 1)).
+Proof.
+  unfold hoare_triple, sa_pure, sa_empty. intros Hnth v' c m m' Hred p.
+  inversion Hred. subst. inversion H; subst. apply Nth_spec in Hnth, H6.
+  rewrite Hnth in *. injection H6 as ?. subst.
+  inversion H0; subst; auto. discriminate_red_Val.
+Qed.
+
+Theorem triple_ref (V : Set) (v : Value V) :
+  @hoare_triple V (Ref v)
+    sa_empty
+    (fun v' c => sa_exists
+      (fun l => sa_star (sa_pure (v' = Lab l /\ c = 1)) (sa_single l v))).
+Proof.
+  unfold hoare_triple, sa_exists, sa_star, sa_single, sa_pure, sa_empty,
+    disjoint_maps.
+  intros v' c m m' Hred p. inversion Hred. subst.
+  inversion H; subst; try discriminate_red_Val.
+  inversion H0; subst; try discriminate_red_Val.
+  repeat eexists. auto.
+Qed.
+
+Theorem triple_deref (V : Set) l (v : Value V) :
+  @hoare_triple V (Deref (Lab l))
+    (sa_single l v)
+    (fun v' c => sa_star (sa_pure (v' = v /\ c = 1)) (sa_single l v)).
+Proof.
+  unfold hoare_triple, sa_star, sa_single, sa_pure, sa_empty, disjoint_maps.
+  intros v' c m m' Hred p. inversion Hred. subst.
+  inversion H; subst; try discriminate_red_Val. apply Lookup_spec in H2.
+  - simpl in *. destruct l as [n]. unfold label_eqb, lift2, lift in *.
+    rewrite Nat.eqb_refl in *. injection H2 as ?. subst.
+    inversion H0; subst; try discriminate_red_Val.
+    repeat eexists. auto.
+  - unfold Is_Valid_Map. simpl. repeat econstructor. auto.
+Qed.
+
+Theorem triple_assign (V : Set) l (v v' : Value V) :
+  @hoare_triple V (Assign (Lab l) v)
+    (sa_single l v')
+    (fun v'' c => sa_star (sa_pure (v'' = U_val /\ c = 1)) (sa_single l v)).
+Proof.
+  unfold hoare_triple, sa_star, sa_single, sa_pure, sa_empty, disjoint_maps.
+  intros v'' c m m' Hred p. inversion Hred. subst.
+  inversion H; subst; try discriminate_red_Val. apply Assignment_spec in H6 as [? ?].
+  - simpl in *. destruct l as [n]. unfold label_eqb, lift2, lift in *.
+    rewrite Nat.eqb_refl in *. subst.
+    inversion H0; subst; try discriminate_red_Val.
+    repeat eexists. auto.
+  - unfold Is_Valid_Map. simpl. repeat econstructor. auto.
+Qed.
+
+Theorem triple_seq (V : Set) (e : Expr V) P Q :
+  hoare_triple e P (fun v c => Q v (1+c)) ->
+  hoare_triple (Seq U_val e) P Q.
+Proof.
+  unfold hoare_triple. intros Hhoare v' c m m' Hred. inversion Hred. subst.
+  apply Hhoare. inversion H; subst; auto. discriminate_red_Val.
+Qed.
+
+Theorem triple_if (V : Set) (b : bool) (e1 e2 : Expr V) P Q :
+  hoare_triple e1 (sa_star (sa_pure (is_true b)) P) (fun v c => Q v (1+c)) ->
+  hoare_triple e2 (sa_star (sa_pure (~ is_true b)) P) (fun v c => Q v (1+c)) ->
+  hoare_triple (If (Bool b) e1 e2) P Q.
+Proof.
+  unfold hoare_triple, sa_star, is_true, sa_pure, sa_empty, disjoint_maps.
+  intros Hhoare1 Hhoare2 v' c m m' Hred p. inversion Hred. subst.
+  destruct b; [eapply Hhoare1 | eapply Hhoare2]; try (repeat eexists; eauto);
+    simpl; inversion H; subst; auto; discriminate_red_Val.
+Qed.
+
+Theorem triple_while (V : Set) (c1 c2 : nat) (e1 e2 : Expr V) P Q :
+  hoare_triple e1
+    P
+    (fun v c1' => sa_exists
+      (fun b => sa_star (sa_pure (v = Bool b /\ c1' = c1)) (Q b))) ->
+  hoare_triple e2
+    (Q true)
+    (fun _ c2' => sa_star (sa_pure (c2' = c2)) P) ->
+  hoare_triple (While e1 e2)
+    P
+    (fun _ c => sa_exists
+      (fun n => sa_star (sa_pure (c = (n * (c1 + 1 + c2)) + c1 + 1)) (Q false))).
+Proof.
+  unfold hoare_triple, sa_exists, sa_star, is_true, sa_pure, sa_empty,
+    disjoint_maps.
+  intros Hhoare1 Hhoare2 v' c m m' Hred p.
+  (** remember (While e1 e2) as e eqn:Hwhile.
+  remember (Val v') as e' eqn:Hval. generalize dependent e'.
+  generalize dependent e.*)
+  induction c as [? IH] using (well_founded_ind lt_wf). inversion Hred. subst.
+  inversion H. subst.
+(*  destruct b; [eapply Hhoare1 | eapply Hhoare2]; try (repeat eexists; eauto);
+    simpl; inversion H; subst; auto; discriminate_red_Val.*)
+Admitted.
+
+(*
+| red_while : forall m e1 e2,
+    R[While e1 e2, m
+      ~~>
+      If e1 (Seq e2 (While e1 e2)) U_val, m]
+
+(* structural rules *)
+| red_app1 : forall m m' e1 e1' e2,
+    R[e1, m ~~> e1', m'] ->
+    R[App e1 e2, m ~~> App e1' e2, m']
+
+| red_app2 : forall m m' (v : Value _) e e',
+    R[e, m ~~> e', m'] ->
+    R[App v e, m ~~> App v e', m']
+
+| red_unop : forall k m m' e e',
+    R[e, m ~~> e', m'] ->
+    R[UnOp k e, m ~~> UnOp k e', m']
+
+| red_binop1 : forall k m m' e1 e1' e2,
+    R[e1, m ~~> e1', m'] ->
+    R[BinOp k e1 e2, m ~~> BinOp k e1' e2, m']
+
+| red_binop2 : forall k m m' (v : Value _) e e',
+    R[e, m ~~> e', m'] ->
+    R[BinOp k v e, m ~~> BinOp k v e', m']
+
+| red_rec_split : forall m m' es es' vs0 e e' es0,
+    L[es  ~~> vals2exprs vs0 | e | es0] ->
+    L[es' ~~> vals2exprs vs0 | e' | es0] ->
+    R[e, m ~~> e', m'] ->
+    R[RecE es, m ~~> RecE es', m']
+
+| red_ref_e : forall m m' e e',
+    R[e, m ~~> e', m'] ->
+    R[Ref e, m ~~> Ref e', m']
+
+| red_deref_e : forall m m' e e',
+    R[e, m ~~> e', m'] ->
+    R[Deref e, m ~~> Deref e', m']
+
+| red_assign1 : forall m m' e1 e1' e2,
+    R[e1, m ~~> e1', m'] ->
+    R[Assign e1 e2, m ~~> Assign e1' e2, m']
+
+| red_assign2 : forall m m' (v : Value _) e e',
+    R[e, m ~~> e', m'] ->
+    R[Assign v e, m ~~> Assign v e', m']
+
+| red_seq1 : forall m m' e1 e1' e2,
+    R[e1, m ~~> e1', m'] ->
+    R[Seq e1 e2, m ~~> Seq e1' e2, m']
+
+| red_cond_if : forall m m' e1 e1' e2 e3,
+    R[e1, m ~~> e1', m'] ->
+    R[If e1 e2 e3, m ~~> If e1' e2 e3, m']
+*)
